\question 
\begin{enumerate}[label=\alph*.]
\item Prove that for independent random variables $X$ and $Y$, 
$\var(X + Y) = \var(X) + \var(Y)$.
\begin{solution}[3 cm]
\begin{equation}
\begin{split}
\var(X + Y) &= \E((X + Y)^2) - \E(X + Y)^2 \\ \nonumber
&= \E(X^2) + \E(Y^2) + 2*\E(XY) - (\E(X) + \E(Y))^2 \\
&= (\E(X^2) - \E(X)^2) + (\E(Y^2)-\E(Y)^2) + 2*\E(XY) - \E(X)*\E(Y) \\
&= \var(X) + \var(Y) + 2 * (\E(XY) - \E(X)\E(Y))
\end{split}
\end{equation}
\end{solution}

\item Is the above result true for non-independent random variables? 
Prove or give a counterexample.
\begin{solution}[4cm]
No! One simple counterexample is $X = Y$. Then
\begin{equation}
\begin{split}
\var(X + Y) &= \var(2x) \\ \nonumber
&= \E((2X)^2) - \E(2X)^2 \\
&= \E(4X^2) - (2*\E(X))^2 \\
&= 4\E(X^2) - 4(\E(X)^2) \\
&= 4 (\E(X^2) - \E(X)^2) \\
&= 4*\var(X)
\end{split}
\end{equation}
\end{solution}

\end{enumerate}