{\tabulinesep=1mm
\begin{tabu}{|p{16cm} |}
\hline
\textit{Goal}: To show $(x^e)^d \equiv x$ mod ($N$), $\forall x \in \{0, 1, \cdots, N-1\}$. 

Since $ed \equiv 1$ mod $(p-1)(q-1)$ (that's how we define $d$), 
$ed = 1 + k(p-1)(q-1)$ for some integer $k$. 
Therefore, $x^{ed} = x^{1 + k(p-1)(q-1)}$\\
$\implies x^{ed} - x = x^{1 + k(p-1)(q-1)} - x = x(x^{k(p-1)(q-1)} - 1)$. \\ 
\textit{Claim}: $p \mid x^{ed} - x$

\textit{Case 1} ($x \not\equiv 0$ mod $p$): \\
According to Fermat's Little Theorem, $x^{p-1} \equiv 1$ mod $p$. 


$\implies (x^{p-1})^{k(q-1)} \equiv 1^{k(q-1)} \mod p$ \\
$\implies x^{k(p-1)(q-1)} - 1 \equiv 0$ mod $p$  \\
$\implies x^{k(p-1)(q-1)+1} - x \equiv 0$ mod $p$\\
$\implies p \mid x^{ed} - x$\\
\textit{Case 2} ($x \equiv 0$ mod $p$): \\
$p \mid x(x^{ed - 1} - 1)$ \\ 
$\implies p \mid x^{ed} - x$\\
By symmetry, $q \mid x^{ed} - x$. Thus, $pq \mid x^{ed} - x$, which means $(x^e)^d \equiv x$ mod ($N$). \\
\hline
\end{tabu}
}